analysis/Analysis/Section_3_5.lean
@@ -418,7 +418,7 @@ theorem SetTheory.Set.Fin.toNat_lt {n:ℕ} (i: Fin n) : i < n := (toNat_spec i).
 theorem SetTheory.Set.Fin.coe_toNat {n:ℕ} (i: Fin n) : ((i:ℕ):Object) = (i:Object) := by
   set j := (i:ℕ); obtain ⟨ h, h':i = Fin_mk n j h ⟩ := toNat_spec i; rw [h']
 
-@[simp]
+@[simp low]
 lemma SetTheory.Set.Fin.coe_inj {n:ℕ} {i j: Fin n} : i = j ↔ (i:ℕ) = (j:ℕ) := by
   constructor
   · simp_all
